src/program_logic/crash_adequacy.v
@@ -21,26 +21,26 @@ Notation wptp s k t := ([∗ list] ef ∈ t, WPC ef @ s; k; ⊤; ⊤ {{ fork_pos
 
 Lemma wpc_step s k e1 σ1 κ κs e2 σ2 efs m Φ Φc :
   prim_step e1 σ1 κ e2 σ2 efs →
-  state_interp σ1 (κ ++ κs) m -∗ WPC e1 @ s; k; ⊤; ⊤ {{ Φ }} {{ Φc }} -∗ NC -∗
+  state_interp σ1 (κ ++ κs) m -∗ WPC e1 @ s; k; ⊤; ⊤ {{ Φ }} {{ Φc }} -∗ NC 1 -∗
   |={⊤}[∅]▷=>
   state_interp σ2 κs (length efs + m) ∗
   WPC e2 @ s; k; ⊤; ⊤ {{ Φ }} {{ Φc }} ∗
   wptp s k efs ∗
-  NC.
+  NC 1.
 Proof.
   rewrite {1}wpc_unfold /wpc_pre. iIntros (?) "Hσ H HNC".
   rewrite (val_stuck e1 σ1 κ e2 σ2 efs) //.
   iMod "H". iDestruct "H" as "(H&_)".
-  iMod ("H" $! σ1 with "Hσ HNC") as "(_&H)".
+  iMod ("H" $! _ σ1 with "Hσ HNC") as "(_&H)".
   iMod ("H" $! e2 σ2 efs with "[//]") as "H".
   by do 2 iModIntro.
 Qed.
 
 Lemma wptp_step s k e1 t1 t2 κ κs σ1 σ2 Φ Φc :
   step (e1 :: t1,σ1) κ (t2, σ2) →
-  state_interp σ1 (κ ++ κs) (length t1) -∗ WPC e1 @ s; k; ⊤; ⊤ {{ Φ }} {{ Φc }}-∗ wptp s k t1 -∗ NC ==∗
+  state_interp σ1 (κ ++ κs) (length t1) -∗ WPC e1 @ s; k; ⊤; ⊤ {{ Φ }} {{ Φc }}-∗ wptp s k t1 -∗ NC 1 ==∗
   ∃ e2 t2', ⌜t2 = e2 :: t2'⌝ ∗
-  |={⊤}[∅]▷=> state_interp σ2 κs (pred (length t2)) ∗ WPC e2 @ s; k; ⊤; ⊤ {{ Φ }} {{ Φc}} ∗ wptp s k t2' ∗ NC.
+  |={⊤}[∅]▷=> state_interp σ2 κs (pred (length t2)) ∗ WPC e2 @ s; k; ⊤; ⊤ {{ Φ }} {{ Φc}} ∗ wptp s k t2' ∗ NC 1.
 Proof.
   iIntros (Hstep) "Hσ He Ht HNC".
   destruct Hstep as [e1' σ1' e2' σ2' efs [|? t1'] t2' ?? Hstep]; simplify_eq/=.
@@ -59,12 +59,12 @@ Qed.
 
 Lemma wptp_steps s k n e1 t1 κs κs' t2 σ1 σ2 Φ Φc :
   nsteps n (e1 :: t1, σ1) κs (t2, σ2) →
-  state_interp σ1 (κs ++ κs') (length t1) -∗ WPC e1 @ s; k; ⊤; ⊤ {{ Φ }} {{ Φc }} -∗ wptp s k t1 -∗ NC -∗
+  state_interp σ1 (κs ++ κs') (length t1) -∗ WPC e1 @ s; k; ⊤; ⊤ {{ Φ }} {{ Φc }} -∗ wptp s k t1 -∗ NC 1 -∗
   |={⊤}[∅]▷=>^n (∃ e2 t2',
     ⌜t2 = e2 :: t2'⌝ ∗
     state_interp σ2 κs' (pred (length t2)) ∗
     WPC e2 @ s; k; ⊤; ⊤ {{ Φ }} {{ Φc }} ∗ wptp s k t2' ∗
-    NC).
+    NC 1).
 Proof.
   revert e1 t1 κs κs' t2 σ1 σ2; simpl.
   induction n as [|n IH]=> e1 t1 κs κs' t2 σ1 σ2 /=.
@@ -78,12 +78,12 @@ Qed.
 
 Lemma wpc_safe E k κs m e σ Φ Φc :
   state_interp σ κs m -∗
-  WPC e @ k ; ⊤ ; E {{ Φ }} {{ Φc }} -∗ NC ={⊤}=∗
+  WPC e @ k ; ⊤ ; E {{ Φ }} {{ Φc }} -∗ NC 1 ={⊤}=∗
   ⌜is_Some (to_val e) ∨ reducible e σ⌝.
 Proof.
   rewrite wpc_unfold /wpc_pre. iIntros "Hσ >(H&_) HNC".
   destruct (to_val e) as [v|] eqn:?; first by eauto.
-  iSpecialize ("H" $! σ [] κs with "Hσ HNC"). rewrite sep_elim_l.
+  iSpecialize ("H" $! _ σ [] κs with "Hσ HNC"). rewrite sep_elim_l.
   iMod (fupd_plain_mask with "H") as %?; eauto.
 Qed.
 
@@ -92,14 +92,14 @@ Lemma wptp_strong_adequacy Φ Φc k κs' s n e1 t1 κs t2 σ1 σ2 :
   state_interp σ1 (κs ++ κs') (length t1) -∗
   WPC e1 @ s; k; ⊤; ⊤ {{ Φ }} {{ Φc }} -∗
   wptp s k t1 -∗
-  NC -∗
+  NC 1 -∗
   |={⊤}[∅]▷=>^(S n) (∃ e2 t2',
     ⌜ t2 = e2 :: t2' ⌝ ∗
     ⌜ ∀ e2, s = NotStuck → e2 ∈ t2 → (is_Some (to_val e2) ∨ reducible e2 σ2) ⌝ ∗
     state_interp σ2 κs' (length t2') ∗
     from_option Φ True (to_val e2) ∗
     ([∗ list] v ∈ omap to_val t2', fork_post v) ∗
-    NC).
+    NC 1).
 Proof.
   iIntros (Hstep) "Hσ He Ht HNC". rewrite Nat_iter_S_r.
   iDestruct (wptp_steps with "Hσ He Ht HNC") as "Hwp"; first done.
@@ -107,7 +107,7 @@ Proof.
   iDestruct 1 as (e2' t2' ?) "(Hσ & Hwp & Ht & HNC)"; simplify_eq/=.
   iMod (fupd_plain_keep_l ⊤
     (⌜ ∀ e2, s = NotStuck → e2 ∈ (e2' :: t2') → (is_Some (to_val e2) ∨ reducible e2 σ2) ⌝)%I
-    (state_interp σ2 κs' (length t2') ∗ WPC e2' @ s; k; ⊤; ⊤ {{ v, Φ v }} {{ Φc }} ∗ wptp s k t2' ∗ NC)%I
+    (state_interp σ2 κs' (length t2') ∗ WPC e2' @ s; k; ⊤; ⊤ {{ v, Φ v }} {{ Φc }} ∗ wptp s k t2' ∗ NC 1)%I
     with "[$Hσ $Hwp $Ht $HNC]") as "(Hsafe&Hσ&Hwp&Hvs&HNC)".
   { iIntros "(Hσ & Hwp & Ht & HNC)" (e' -> He').
     apply elem_of_cons in He' as [<-|(t1''&t2''&->)%elem_of_list_split].
@@ -128,7 +128,7 @@ Lemma wptp_strong_crash_adequacy Φ Φc κs' s k n e1 t1 κs t2 σ1 σ2 :
   state_interp σ1 (κs ++ κs') (length t1) -∗
   WPC e1 @ s; k; ⊤; ⊤ {{ Φ }} {{ Φc }} -∗
   wptp s k t1 -∗
-  NC -∗
+  NC 1 -∗
   |={⊤}[∅]▷=>^(S n) |={⊤,∅}=> ▷ (∃ e2 t2',
     ⌜ t2 = e2 :: t2' ⌝ ∗
     Φc ∗ state_interp σ2 κs' (length t2') ∗ C).
@@ -139,7 +139,7 @@ Proof.
   iDestruct 1 as (e2' t2' ?) "(Hσ & Hwp & Ht & HNC)"; simplify_eq/=.
   iMod (fupd_plain_keep_l ⊤
     (⌜ ∀ e2, s = NotStuck → e2 ∈ (e2' :: t2') → (is_Some (to_val e2) ∨ reducible e2 σ2) ⌝)%I
-    (state_interp σ2 κs' (length t2') ∗ WPC e2' @ s; k; ⊤; ⊤ {{ v, Φ v }} {{ Φc }} ∗ wptp s k t2' ∗ NC)%I
+    (state_interp σ2 κs' (length t2') ∗ WPC e2' @ s; k; ⊤; ⊤ {{ v, Φ v }} {{ Φc }} ∗ wptp s k t2' ∗ NC 1)%I
     with "[$Hσ $Hwp $Ht $HNC]") as "(Hsafe&Hσ&Hwp&Hvs&HNC)".
   { iIntros "(Hσ & Hwp & Ht & HNC)" (e' -> He').
     apply elem_of_cons in He' as [<-|(t1''&t2''&->)%elem_of_list_split].
